Fixup for traits

Source/DafnyCore/Backends/Dafny/DafnyCodeGenerator.cs
@@ -877,7 +877,7 @@ namespace Microsoft.Dafny.Compilers {
     }
 
     protected override void TypeArgDescriptorUse(bool isStatic, bool lookasideBody, TopLevelDeclWithMembers cl, out bool needsTypeParameter, out bool needsTypeDescriptor) {
-      needsTypeParameter = true;
+      needsTypeParameter = false;
       needsTypeDescriptor = false;
     }
 
